cedar-lean/Cedar/Thm/Validation/Levels.lean
@@ -27,9 +27,127 @@ open Cedar.Data
 open Cedar.Spec
 open Cedar.Validation
 
+theorem entities_attrs_then_find? {entities: Entities} {attrs : Map Attr Value} {uid : EntityUID}
+  (he : entities.attrs uid = .ok attrs)
+  : ∃ ed, entities.find? uid = some ed ∧ ed.attrs = attrs
+:= by sorry
+
+theorem entities_find?_then_attrs {entities: Entities} {ed : EntityData} {uid : EntityUID}
+  (he : entities.find? uid = some ed)
+  : .ok ed.attrs = entities.attrs uid
+:= by sorry
+
+-- theorem entities_attrs_iff_find? {entities: Entities} {attrs : Map Attr Value} {uid : EntityUID}
+--   : (entities.attrs uid = .ok attrs) ↔ (∃ ed, entities.find? uid = some ed ∧ ed.attrs = attrs)
+-- := by sorry
+
+theorem check_level_root_invariant (n n' : Nat) (e : TypedExpr)
+  : (checkLevel e n).root = (checkLevel e n').root
+:= by
+  unfold checkLevel
+  cases e <;> simp
+  case ite | unaryApp =>
+    simp [check_level_root_invariant n n']
+  case binaryApp op _ _ _ =>
+    cases op
+    case mem | getTag | hasTag =>
+      simp [check_level_root_invariant (n - 1) (n' - 1)]
+    all_goals { simp [check_level_root_invariant n n'] }
+  case getAttr e _ _ | hasAttr e _ _ =>
+    cases e.typeOf
+    case entity =>
+      simp [check_level_root_invariant (n - 1) (n' - 1)]
+    all_goals { simp [check_level_root_invariant n n'] }
+  -- Hopefully should be trivial
+  case set es _ | call es _ => sorry
+  case record a => sorry
+
+theorem check_level_succ {e : TypedExpr} {n : Nat}
+  (h₁ : (checkLevel e n).checked)
+  : (checkLevel e (1 + n)).checked
+:= by
+  cases e <;> try (simp [checkLevel] at h₁ ; simp [checkLevel])
+  case ite | and | or | unaryApp =>
+    simp [h₁, check_level_succ]
+  case binaryApp op e₀ _ _ =>
+    cases op <;> (
+      simp [checkLevel] at h₁
+      simp [checkLevel]
+      simp [h₁, check_level_succ]
+    )
+    case mem | hasTag | getTag =>
+      repeat constructor
+      · have h₂ := check_level_root_invariant (1 + n - 1) (n - 1)
+        simp [h₂, h₁]
+      · omega
+      · have h₂ : (1 + n - 1) = (1 + (n - 1)) := by omega
+        simp [h₁, h₂, check_level_succ]
+  case hasAttr e _ _ | getAttr e _ _ =>
+    split at h₁
+    · simp [checkLevel] at h₁
+      simp [checkLevel]
+      repeat constructor
+      · have h₂ := check_level_root_invariant (1 + n - 1) (n - 1)
+        simp [h₂, h₁]
+      · omega
+      · have h₂ : (1 + n - 1) = (1 + (n - 1)) := by omega
+        simp [h₁, h₂, check_level_succ]
+    · simp [h₁, check_level_succ]
+  -- should be trivial
+  case set | call => sorry
+  case record => sorry
+
+theorem slice_at_level_inner_succ {n: Nat} {work : Set EntityUID} {uid : EntityUID} {entities : Entities} {slice₀ slice₁ : Set EntityUID}
+  (hs₀ : slice₀ = Entities.sliceAtLevel.sliceAtLevel entities work n)
+  (hs₁ : slice₁ = Entities.sliceAtLevel.sliceAtLevel entities work (1 + n))
+  (he₀ : uid ∈ slice₀ )
+  : uid ∈ slice₁
+:= by
+  cases n
+  case zero =>
+    replace hs₀ : some slice₀ = some ∅ := by
+      simp [hs₀, Entities.sliceAtLevel, Entities.sliceAtLevel.sliceAtLevel]
+    injections hs₀
+    rw [hs₀] at he₀
+    contradiction
+  case succ n =>
+    unfold Entities.sliceAtLevel.sliceAtLevel at hs₀ hs₁
+    simp at hs₀ hs₁
+    have h₁ : (1 + (n + 1) - 1) = (1 + n) := by omega
+    rw [h₁] at hs₁
+    cases hm : List.mapM (Map.find? entities) work.elts <;> simp [hm] at hs₀ hs₁
+    rename_i sliceₙ
+    cases hrs₀ : (Entities.sliceAtLevel.sliceAtLevel entities (flatten_union (List.map EntityData.sliceEUIDs sliceₙ)) n) <;> simp [hrs₀] at hs₀
+    cases hrs₁ : (Entities.sliceAtLevel.sliceAtLevel entities (flatten_union (List.map EntityData.sliceEUIDs sliceₙ)) (1 + n)) <;> simp [hrs₁] at hs₁
+    rename_i slice₀' slice₁'
+    subst slice₀ slice₁
+    have ⟨ hi₀, _ ⟩ := Set.mem_union_iff_mem_or work slice₀' uid
+    specialize hi₀ he₀
+    cases hi₀
+    case inl hi₀ =>
+      have ⟨ _, hi₁ ⟩ := Set.mem_union_iff_mem_or work slice₁' uid
+      simp [hi₁, hi₀]
+    case inr hi₀ =>
+      have ⟨ _, hi₁ ⟩ := Set.mem_union_iff_mem_or work slice₁' uid
+      symm at hrs₀ hrs₁
+      simp [hi₁, slice_at_level_inner_succ hrs₀ hrs₁ hi₀]
+
+theorem slice_at_level_succ {n: Nat} {request : Request} {uid : EntityUID} {data : EntityData} {entities : Entities} {slice₀ slice₁ : Entities}
+  (hs₀ : slice₀ = Entities.sliceAtLevel entities request n)
+  (hs₁ : slice₁ = Entities.sliceAtLevel entities request (1 + n))
+  (he₀ : slice₀.find? uid = some data)
+  : slice₁.find? uid = some data
+:= by sorry
+
+theorem not_entities_attrs_then_not_slice_attrs {n: Nat} {request : Request} {uid : EntityUID} {e : Error} {entities slice : Entities}
+  (hs : slice = Entities.sliceAtLevel entities request n)
+  (hse : entities.attrs uid = .error e)
+  : slice.attrs uid = .error e
+:= by sorry
+
 theorem typed_at_level_inversion {e : Expr} {c₀: Capabilities} {env : Environment} {n : Nat} :
   typedAtLevel e c₀ env n ->
-  ∃ tx c₁, typeOf e c₀ env = .ok (tx, c₁) ∧ checkLevel tx n
+  ∃ tx c₁, typeOf e c₀ env = .ok (tx, c₁) ∧ (checkLevel tx n).checked
 := by
   unfold typedAtLevel
   split
@@ -39,7 +157,7 @@ theorem typed_at_level_inversion {e : Expr} {c₀: Capabilities} {env : Environm
   · simp
 
 theorem typed_at_level_def {e : Expr} {tx : TypedExpr} {c₀ c₁: Capabilities} {env : Environment} {n : Nat} :
-  typeOf e c₀ env = .ok (tx, c₁) → checkLevel tx n →
+  typeOf e c₀ env = .ok (tx, c₁) → (checkLevel tx n).checked →
   typedAtLevel e c₀ env n
 := by
   intros h₁
@@ -47,38 +165,40 @@ theorem typed_at_level_def {e : Expr} {tx : TypedExpr} {c₀ c₁: Capabilities}
   rw [h₁]
   simp
 
-def TypedAtLevelIsSound₀ (e : Expr) : Prop := ∀ {c : Capabilities} {env :Environment} {request : Request} {entities : Entities},
-  -- slice = entities.sliceAtLevel request 0 →
+def TypedAtLevelIsSound (e : Expr) : Prop := ∀ {n : Nat} {c : Capabilities} {env :Environment} {request : Request} {entities slice : Entities},
+  slice = entities.sliceAtLevel request n →
   CapabilitiesInvariant c request entities →
   RequestAndEntitiesMatchEnvironment env request entities →
-  typedAtLevel e c env 0 →
-  evaluate e request entities = evaluate e request Map.empty
+  typedAtLevel e c env n →
+  evaluate e request entities = evaluate e request slice
 
-theorem level_based_slicing_is_sound_if₀ {c t e : Expr} {c₀ c₁: Capabilities} {env : Environment} {request : Request} {entities : Entities}
+theorem level_based_slicing_is_sound_if {c t e : Expr} {n : Nat} {c₀ c₁: Capabilities} {env : Environment} {request : Request} {entities slice : Entities}
+  (hs : slice = entities.sliceAtLevel request n)
   (hc : CapabilitiesInvariant c₀ request entities)
   (h₂ : RequestAndEntitiesMatchEnvironment env request entities)
   (h₃ : typeOf (.ite c t e) c₀ env = Except.ok (tx, c₁))
-  (h₄ : checkLevel tx 0 = true)
-  (ihc : TypedAtLevelIsSound₀ c)
-  (iht : TypedAtLevelIsSound₀ t)
-  (ihe : TypedAtLevelIsSound₀ e)
-  : evaluate (.ite c t e) request entities = evaluate (.ite c t e) request Map.empty
+  (h₄ : (checkLevel tx n).checked = true)
+  (ihc : TypedAtLevelIsSound c)
+  (iht : TypedAtLevelIsSound t)
+  (ihe : TypedAtLevelIsSound e)
+  : evaluate (.ite c t e) request entities = evaluate (.ite c t e) request slice
 := by
-    have ⟨ty₁, bty₁, c₁, ty₂, c₂, ty₃, c₃, h₅, h₆, h₇ ⟩ := type_of_ite_inversion h₃
-    have ⟨ hgc, v, h₁₃, h₁₄ ⟩ := type_of_is_sound hc h₂ h₅
-    rw [h₆] at h₁₄
-    split at h₇
-    · replace ⟨h₇, h₈, _⟩ := h₇
-      subst h₈
+    have ⟨ty₁, bty₁, c₁, ty₂, c₂, ty₃, c₃, h₅, h₆, h₇, h₈ ⟩ := type_of_ite_inversion h₃
+    have ⟨ hgc, v, h₁₃, h₁₄ ⟩ := type_of_is_sound hc h₂ h₆
+    rw [h₇] at h₁₄
+    split at h₈
+    · replace ⟨h₇, h₈, h₉⟩ := h₈
+      subst h₉
       replace h₁₄ := instance_of_ff_is_false h₁₄
       subst h₁₄
+      rw [h₅] at h₄
       simp only [checkLevel, Bool.and_eq_true] at h₄
       have ⟨ ⟨ hl₄, _ ⟩,  hr₄⟩ := h₄
-      specialize ihc hc h₂ (typed_at_level_def h₅ hl₄)
-      specialize ihe hc h₂ (typed_at_level_def h₇ hr₄)
+      specialize ihc hs hc h₂ (typed_at_level_def h₆ hl₄)
+      specialize ihe hs hc h₂ (typed_at_level_def h₇ hr₄)
       simp only [evaluate]
       rw [ihc, ihe]
-      cases h₁₂ : Result.as Bool (evaluate c request Map.empty) <;> simp only [Except.bind_err, Except.bind_ok]
+      cases h₁₂ : Result.as Bool (evaluate c request slice) <;> simp only [Except.bind_err, Except.bind_ok]
       simp only [Result.as, Coe.coe, Value.asBool] at h₁₂
       split at h₁₂ <;> try simp only [reduceCtorEq] at h₁₂
       split at h₁₂ <;> try simp only [reduceCtorEq, Except.ok.injEq] at h₁₂
@@ -87,16 +207,17 @@ theorem level_based_slicing_is_sound_if₀ {c t e : Expr} {c₀ c₁: Capabiliti
       simp only [EvaluatesTo, ihc, h₁₅, reduceCtorEq, Except.ok.injEq, Value.prim.injEq, Prim.bool.injEq, false_or] at h₁₃
       subst h₁₃
       simp
-    · replace ⟨h₇, h₈, _⟩ := h₇
-      subst h₈
+    · replace ⟨h₇, h₈, h₉⟩ := h₈
+      subst h₉
       replace h₁₄ := instance_of_tt_is_true h₁₄
       subst h₁₄
+      rw [h₅] at h₄
       simp only [checkLevel, Bool.and_eq_true] at h₄
-      have ⟨ ⟨ hl₄, _ ⟩,  hr₄⟩ := h₄
-      specialize ihc hc h₂ (typed_at_level_def h₅ hl₄)
+      have ⟨ ⟨ hl₄, hr₄ ⟩,  _⟩ := h₄
+      specialize ihc hs hc h₂ (typed_at_level_def h₆ hl₄)
       simp only [evaluate]
       rw [ihc]
-      cases h₁₂ : Result.as Bool (evaluate c request Map.empty) <;> simp only [Except.bind_err, Except.bind_ok]
+      cases h₁₂ : Result.as Bool (evaluate c request slice) <;> simp only [Except.bind_err, Except.bind_ok]
       simp only [Result.as, Coe.coe, Value.asBool] at h₁₂
       split at h₁₂ <;> try simp only [reduceCtorEq] at h₁₂
       split at h₁₂ <;> try simp only [reduceCtorEq, Except.ok.injEq] at h₁₂
@@ -105,16 +226,16 @@ theorem level_based_slicing_is_sound_if₀ {c t e : Expr} {c₀ c₁: Capabiliti
       simp only [EvaluatesTo, ihc, h₁₅, reduceCtorEq, Except.ok.injEq, Value.prim.injEq, Prim.bool.injEq, false_or] at h₁₃
       subst h₁₃
       simp only [GuardedCapabilitiesInvariant, ihc, h₁₅, forall_const] at hgc
-      specialize iht (capability_union_invariant hc hgc) h₂ (typed_at_level_def h₇ hr₄)
+      specialize iht hs (capability_union_invariant hc hgc) h₂ (typed_at_level_def h₇ hr₄)
       simp [iht]
-    · replace ⟨h₇, h₈, h₉, h₁₀, _⟩ := h₇
-      rw [h₉] at h₄
+    · replace ⟨h₇, h₈, h₉, h₁₀⟩ := h₈
+      rw [h₅] at h₄
       simp only [checkLevel, Bool.and_eq_true] at h₄
       have ⟨⟨ ha₄, hb₄ ⟩, hc₄ ⟩ := h₄
-      specialize ihc hc h₂ (typed_at_level_def h₅ ha₄)
-      specialize ihe hc h₂ (typed_at_level_def h₈ hc₄)
+      specialize ihc hs hc h₂ (typed_at_level_def h₆ ha₄)
+      specialize ihe hs hc h₂ (typed_at_level_def h₈ hc₄)
       simp only [ihc, ihe, evaluate]
-      cases h₁₂ : Result.as Bool (evaluate c request Map.empty) <;> simp only [Except.bind_err, Except.bind_ok]
+      cases h₁₂ : Result.as Bool (evaluate c request slice) <;> simp only [Except.bind_err, Except.bind_ok]
       simp only [Result.as, Coe.coe, Value.asBool] at h₁₂
       split at h₁₂ <;> try simp only [reduceCtorEq] at h₁₂
       split at h₁₂ <;> try simp only [reduceCtorEq, Except.ok.injEq] at h₁₂
@@ -124,136 +245,678 @@ theorem level_based_slicing_is_sound_if₀ {c t e : Expr} {c₀ c₁: Capabiliti
       case false => simp
       case true =>
         simp only [GuardedCapabilitiesInvariant, ihc, h₁₄, forall_const] at hgc
-        specialize iht (capability_union_invariant hc hgc) h₂ (typed_at_level_def h₇ hb₄)
+        specialize iht hs (capability_union_invariant hc hgc) h₂ (typed_at_level_def h₇ hb₄)
         simp [iht]
 
-theorem level_based_slicing_is_sound₀ {e : Expr} {c : Capabilities} {env : Environment} {request : Request} {entities : Entities}
-  -- slice = entities.sliceAtLevel request 0 →
+theorem mapm_elem {α β: Type} {l : List α} {l' : List β} {f : α → Option β} {e: α}
+  (h₁ : List.mapM f l = l')
+  (h₂ : e ∈ l)
+  : ∃ e', f e = some e' ∧ e' ∈ l'
+:= by
+  have ⟨ y, h₃, h₄ ⟩ := List.mapM_some_implies_all_some h₁ e h₂
+  exists y
+
+theorem mapm_pair_lookup  {α γ : Type} [BEq α] [LawfulBEq α] {l : List α} {l' : List (α × γ)} {f : α → Option (α × γ)} {e: α}
+  (h₁ : List.mapM f l = some l')
+  (h₂ : e ∈ l)
+  (hf : ∀ e, match f e with
+    | some e' => e'.fst = e
+    | none => True)
+  : ∃ e', f e = some e' ∧  l'.lookup e'.fst = some e'.snd
+:= by
+  cases l
+  case nil => contradiction
+  case cons h t =>
+    cases h₃ : f h <;>
+    cases h₄ : List.mapM f t <;>
+    simp only [h₃, h₄, List.mapM_cons, Option.pure_def, Option.bind_none_fun, Option.bind_some_fun, Option.some.injEq, reduceCtorEq] at h₁
+    subst h₁
+    simp only [List.mem_cons] at h₂
+    cases h₂
+    case _ h₂ =>
+      simp [h₂, h₃, List.lookup]
+    case _ h₂ =>
+      have ⟨ e'', ih₁, ih₂ ⟩ := mapm_pair_lookup h₄ h₂ hf
+      have fh₁ := hf h ; rw [h₃] at fh₁ ; subst fh₁
+      have fh₂ := hf e ; rw [ih₁] at fh₂ ; subst fh₂
+      simp only [ih₁,ih₂, Option.some.injEq, List.lookup, exists_eq_left']
+      split
+      · rename_i h₅
+        simp only [beq_iff_eq] at h₅
+        simp only [←h₅, ih₁, Option.some.injEq] at h₃
+        rw [h₃]
+      · simp
+
+theorem euid_in_work_then_in_slice
+  (hw : euid ∈ work)
+  (hs : some slice = Entities.sliceAtLevel.sliceAtLevel entities work n)
+  (hn : n > 0)
+  : euid ∈ slice
+:= by
+  unfold Entities.sliceAtLevel.sliceAtLevel at hs
+  split at hs
+  case isTrue hn' =>
+    replace hn : (n == 0) = false :=
+      by simp only [beq_eq_false_iff_ne, ne_eq]; omega
+    simp [hn] at hn'
+  case isFalse =>
+    cases h₁ :
+      List.mapM (Map.find? entities) work.elts
+    <;> simp [h₁] at hs
+    rename_i eds
+    cases h₂ :
+      List.mapM (fun x => Entities.sliceAtLevel.sliceAtLevel entities x.sliceEUIDs (n - 1)) eds
+    <;> simp [h₂] at hs
+    rename_i slice'
+    subst hs
+    have ⟨ _, hc ⟩ := Set.mem_union_iff_mem_or work (flatten_union slice') euid
+    apply hc
+    simp [hw]
+
+/-
+theorem slice_at_zero_empty_inner
+  (hs : some slice = Entities.sliceAtLevel.sliceAtLevel entities work 0)
+  : slice = ∅
+:= by
+  simp only [Entities.sliceAtLevel.sliceAtLevel, beq_self_eq_true, ↓reduceIte, Option.some.injEq] at hs
+  exact hs
+
+theorem slice_at_zero_empty {request : Request} {entities slice : Entities}
+  (hs : some slice = Entities.sliceAtLevel entities request 0)
+  : slice = Map.empty
+:= by
+  simp [Entities.sliceAtLevel] at hs
+  cases h₁ : Entities.sliceAtLevel.sliceAtLevel entities request.sliceEUIDs 0 <;> simp [h₁] at hs
+  symm at h₁
+  simp [hs, slice_at_zero_empty_inner h₁, Map.empty, Map.make, List.canonicalize]
+-/
+
+/--
+theorem slice_at_1_has_entity_inner
+  {e: Expr} {tx : TypedExpr} {c c' : Capabilities} {env : Environment} {request : Request} {work : Set EntityUID} {euid : EntityUID} {data : EntityData} {entities : Entities} {slice : List (EntityUID × EntityData)}
+  (hs : slice = Entities.sliceAtLevel.sliceAtLevel entities work 1)
+  (hc : CapabilitiesInvariant c request entities)
+  (hr : RequestAndEntitiesMatchEnvironment env request entities)
+  (ht : typeOf e c env = .ok (tx, c'))
+  (hl : checkLevel tx 0 = LevelCheckResult.mk true true)
+  (he : evaluate e request entities = Except.ok (Value.prim (Prim.entityUID euid)))
+  (hf : entities.find? euid = .some data) :
+  slice.lookup euid = .some data
+:= by
+  cases e
+  case lit =>
+    simp [evaluate] at he
+    subst he
+    simp [typeOf] at ht
+    unfold typeOfLit at ht
+    simp only at ht
+    cases h₁ : (env.ets.contains euid.ty || env.acts.contains euid)
+    · simp [h₁, err] at ht
+    · simp [h₁, ok] at ht
+      simp [checkLevel, ←ht] at hl
+  case var v => sorry
+  /-
+    cases v <;> simp [evaluate] at he <;> subst he
+    all_goals {
+      simp [Entities.sliceAtLevel.sliceAtLevel] at hs
+      have ⟨ e'', h₂, h₃⟩ := mapm_pair_lookup hs hw
+      simp [hf] at h₂
+      subst h₂
+      simp at h₃
+      exact h₃
+    }
+  -/
+  case ite i t e =>
+    have ⟨ty₁, bty₁, c₁, ty₂, c₂, ty₃, c₃, h₂, h₃, h₄, h₅ ⟩ := type_of_ite_inversion ht
+    have hmk : ∀ r, r = LevelCheckResult.mk r.checked r.root := by simp
+    have hl₂ : checkLevel ty₂ 0 = { checked := true, root := true } := by
+      rw [hmk (checkLevel ty₂ 0)]
+      rw [h₂] at hl
+      simp only [checkLevel, LevelCheckResult.mk.injEq,Bool.and_eq_true] at hl
+      simp [hl]
+    have hl₃ : checkLevel ty₃ 0 = { checked := true, root := true } := by
+      rw [hmk (checkLevel ty₃ 0)]
+      rw [h₂] at hl
+      simp only [checkLevel, LevelCheckResult.mk.injEq,Bool.and_eq_true] at hl
+      simp [hl]
+    simp [evaluate] at he
+    cases h₁ : Result.as Bool (evaluate i request entities) <;> simp [h₁] at he
+    split at he
+    case isTrue =>
+      split at h₅
+      · sorry
+      · replace ⟨ h₅, _, _ ⟩ := h₅
+        have huc : CapabilitiesInvariant (c ∪ c₁) request entities := by sorry
+        exact slice_at_1_has_entity_inner hs huc hr h₅ hl₂ he hf
+      · replace ⟨ h₅, _, _, _ ⟩ := h₅
+        have huc : CapabilitiesInvariant (c ∪ c₁) request entities := by sorry
+        exact slice_at_1_has_entity_inner hs huc hr h₅ hl₂ he hf
+    case isFalse =>
+      split at h₅
+      · replace ⟨ h₅, _, _ ⟩ := h₅
+        exact slice_at_1_has_entity_inner hs hc hr h₅ hl₃ he hf
+      · sorry
+      · replace ⟨ _, h₅, _, _ ⟩ := h₅
+        exact slice_at_1_has_entity_inner hs hc hr h₅ hl₃ he hf
+  case and => sorry
+  case or => sorry
+  case unaryApp o e =>
+    simp [evaluate, apply₁] at he
+    cases h₁ : evaluate e request entities <;> simp [h₁] at he
+    split at he <;> try simp at he
+    simp [intOrErr] at he
+    split at he <;> simp at he
+  case binaryApp => sorry
+  case getAttr e a =>
+    have ⟨ _, _, _, _, h₁, h₂ ⟩ := type_of_getAttr_inversion ht
+    cases h₂
+    · rename_i h₂ ; replace ⟨ _, h₂⟩ := h₂
+      rw [h₁] at hl
+      simp [checkLevel, h₂] at hl
+    · sorry
+  case hasAttr => sorry
+  case set => sorry
+  case record => sorry
+  case call => sorry
+--/
+
+def ReachableIn (es : Entities) (start : Set EntityUID) (finish : EntityUID) (level : Nat) : Prop :=
+    if level == 0 then False else
+      finish ∈ start ∨
+        ∃ uid ∈ start, ∃ ed,
+          some ed  = es.find? uid ∧
+          ReachableIn es ed.sliceEUIDs finish (level - 1)
+    termination_by level
+    decreasing_by
+      rename_i h₁
+      simp only [beq_iff_eq] at h₁
+      omega
+
+def EuidInValue (v : Value) (path : List Attr) (euid : EntityUID) : Prop :=
+  match path with
+  | [] =>
+    match v with
+    | .prim (.entityUID euid') => euid' = euid
+    | _ => False
+  | a :: path' =>
+    match v with
+    | .record attrs =>
+      match attrs.find? a with
+      | .some v' => EuidInValue v' path' euid
+      | .none => False
+    | _ => False
+
+theorem mapm_mem
+  (h₁ : some l' = List.mapM f l)
+  (h₂ : e ∈ l)
+  :  ∃ e', some e' = f e ∧ e' ∈ l'
+:= by sorry
+
+theorem mem_flatten_union_iff_mem_any {α : Type} [LT α] [DecidableLT α] {ll : List (Set α)} {e : α}
+  : e ∈ flatten_union ll ↔ ∃ l ∈ ll, e ∈ l
+:= by sorry
+
+theorem slice_contains_reachable
+  {n: Nat}
+  {work : Set EntityUID} {euid : EntityUID} {entities : Entities} {slice : Set EntityUID}
+  (hw : ReachableIn entities work euid (1 + n))
+  (hs : some slice = Entities.sliceAtLevel.sliceAtLevel entities work (1 + n))
+  (h₅ : entities.contains euid) :
+  euid ∈ slice
+:= by
+  cases n
+  case zero =>
+    simp [ReachableIn] at hw
+    exact euid_in_work_then_in_slice hw hs (by simp)
+  case succ =>
+    unfold ReachableIn at hw
+    simp at hw
+    cases hw
+    case inl hw =>
+      exact euid_in_work_then_in_slice hw hs (by omega)
+    case inr hw =>
+      replace ⟨ euid', hi, ed, hf, hw ⟩ := hw
+      rename_i n'
+      have h₆ : (1 + (n' + 1) - 1) = 1 + n' := by omega
+      rw [h₆] at hw
+      unfold Entities.sliceAtLevel.sliceAtLevel at hs
+      simp at hs
+      cases h₇ : (List.mapM (Map.find? entities) work.elts) <;> simp [h₇] at hs
+      rename_i eds
+      cases h₈ : Option.map flatten_union (List.mapM (fun x => Entities.sliceAtLevel.sliceAtLevel entities x.sliceEUIDs (1 + (n' + 1) - 1)) eds) <;> simp [h₈] at hs
+      subst hs
+      rename_i slice'
+      cases h₉ : List.mapM (fun x => Entities.sliceAtLevel.sliceAtLevel entities x.sliceEUIDs (1 + (n' + 1) - 1)) eds <;> simp [h₉] at h₈
+      subst h₈
+      rw [Set.mem_union_iff_mem_or]
+      right
+      symm at h₇
+      have ⟨ e', h₁₀, h₁₁⟩ := mapm_mem h₇ hi
+      rw [←h₁₀] at hf
+      injections hf
+      subst hf
+      cases h₁₂ : (Entities.sliceAtLevel.sliceAtLevel entities ed.sliceEUIDs (1 + n'))
+      case none =>
+        -- `ed ∈ eds` by `h11` and we know mapm of this over all elements `eds`
+        -- is `some`, so this element must be `some`
+        sorry
+      case some =>
+        symm at h₁₂
+        have ih := slice_contains_reachable hw h₁₂ h₅
+        rw [h₆] at h₉
+        rename_i ed_slice
+        symm at h₉
+        have ⟨ e'', h₁₃, h₁₄⟩ := mapm_mem h₉ h₁₁
+        rw [←h₁₃] at h₁₂
+        injections h₁₂
+        subst h₁₂
+        rw [mem_flatten_union_iff_mem_any]
+        exists ed_slice
+
+theorem map_find_mapm_value {α β : Type} [LT α] [DecidableLT α] [BEq α] {ks : Set α} {k : α} {kvs : List (α × β)} {fn : α → Option β}
+  (h₁ : some kvs = List.mapM (λ k => (fn k).bind λ v => (some (k, v))) ks.elts)
+  (h₂ : k ∈ ks)
+  : (Map.make kvs).find? k = fn k
+:= by
+  cases h₃ : ks.elts
+  case nil =>
+    have hcontra : List.Mem k [] := by
+      simp only [Membership.mem, h₃] at h₂
+      exact h₂
+    contradiction
+  case cons h t =>
+    simp [h₃] at h₁
+    cases h₄ : ((fn h).bind fun v => some (h, v)) <;> simp [h₄] at h₁
+    cases h₅ : (List.mapM (fun k => (fn k).bind fun v => some (k, v)) t) <;> simp [h₅] at h₁
+    subst h₁
+    simp only [Membership.mem, h₃] at h₂
+    cases h₂
+    case head =>
+      cases h₆ : (fn k) <;> simp [h₆] at h₄
+      subst h₄
+      sorry
+    case tail h₂ =>
+      symm at h₅
+      sorry
+
+theorem attrs_then_find {entities : Entities} {euid : EntityUID} :
+  (entities.attrs euid).isOk → entities.contains euid
+:= by sorry
+
+theorem reachable_succ {n : Nat} {euid : EntityUID} {start : Set EntityUID} {entities : Entities}
+  (hr : ReachableIn entities start euid n)
+  : ReachableIn entities start euid (1 + n)
+:= by
+  unfold ReachableIn at hr ⊢
+  split at hr
+  · contradiction
+  · rename_i hn
+    have hsn : ((1 + n == 0) = true) = False := by simp
+    simp only [hsn, ↓reduceIte]
+    cases hr
+    case inl hr => simp [hr]
+    case inr hr =>
+      right
+      have ⟨ euid', hs, ed', hrl, hrr ⟩ := hr ; clear hr
+      exists euid'
+      simp only [hs, true_and]
+      exists ed'
+      simp only [hrl, true_and]
+      simp only [beq_iff_eq] at hn
+      have hterm : n - 1 < n := by omega
+      have ih := reachable_succ hrr
+      replace hn : (1 + n - 1) = (1 + (n - 1)) := by omega
+      simp [hn, ih]
+termination_by n
+
+theorem reachable_ancestor_step {n : Nat} {euid euid' : EntityUID} {start : Set EntityUID} {entities : Entities} {ed : EntityData}
+  (hr : ReachableIn entities start euid n)
+  (he : .some ed = entities.find? euid)
+  (he' : euid' ∈ ed.ancestors) :
+  ReachableIn entities start euid' (1 + n)
+:= by sorry
+
+theorem reachable_tag_step {n : Nat} {euid euid' : EntityUID} {start : Set EntityUID} {entities : Entities} {ed : EntityData} {t : Tag}
+  (hr : ReachableIn entities start euid n)
+  (he : .some ed = entities.find? euid)
+  (he' : .some (.prim (.entityUID euid')) = ed.tags.find? t) :
+  ReachableIn entities start euid' (1 + n)
+:= by sorry
+
+theorem reachable_attr_step {n : Nat} {euid euid' : EntityUID} {start : Set EntityUID} {entities : Entities} {ed : EntityData} {a : Attr}
+  (hr : ReachableIn entities start euid n)
+  (he₁: .some ed = entities.find? euid)
+  (he₂ : .some v = ed.attrs.find? a)
+  (he₃ : ∃ path, EuidInValue v path euid' ) :
+  -- (he' : .some (.prim (.entityUID euid')) = ed.attrs.find? a) :
+  ReachableIn entities start euid' (1 + n)
+:= by
+  unfold ReachableIn at hr ⊢
+  split at hr
+  · contradiction
+  · rename_i hn
+    have hsn : ((1 + n == 0) = true) = False := by simp
+    simp only [hsn, ↓reduceIte]
+    cases hr
+    case inl hr =>
+      right
+      exists euid
+      simp only [hr, true_and]
+      exists ed
+      simp only [he₁, true_and]
+      have hn' : (1 + n - 1) = n := by omega
+      rw [hn']
+      unfold ReachableIn
+      simp only [hn, Bool.false_eq_true, ↓reduceIte]
+      left
+      unfold EntityData.sliceEUIDs
+      rw [Set.mem_union_iff_mem_or]
+      left
+      rw [mem_flatten_union_iff_mem_any]
+      exists (Value.prim (Prim.entityUID euid')).sliceEUIDs
+      constructor
+      case left =>
+        simp
+        exists Value.prim (Prim.entityUID euid')
+        simp only [and_true]
+        -- If exists `a` where `ed.attrs.find? a` is `some v` (`he'`) then `v` in `ed.attrs.values`
+        sorry
+      case right =>
+        simp [Value.sliceEUIDs, Set.mem_singleton]
+    case inr hr =>
+      have ⟨ euid'', hs, ed'', hrl, hrr ⟩ := hr ; clear hr
+      right
+      exists euid''
+      simp only [hs, true_and]
+      exists ed''
+      simp only [hrl, true_and]
+      have hn' : (1 + n - 1) = (1 + (n - 1)) := by simp at hn; omega
+      rw [hn']
+      exact reachable_attr_step hrr he₁ he₂ he₃
+
+theorem in_val_then_val_slice
+  (hv : EuidInValue v path euid)
+  : euid ∈ v.sliceEUIDs
+:= by
+  cases v
+  case prim p =>
+    unfold EuidInValue at hv
+    cases p
+    case entityUID =>
+      split at hv <;> simp only at hv
+      simp [hv, Value.sliceEUIDs, Set.mem_singleton]
+    all_goals { split at hv <;> contradiction }
+  case record attrs =>
+    unfold EuidInValue at hv
+    split at hv <;> simp at hv
+    rename_i path a path'
+    split at hv <;> try contradiction
+    rename_i v ha
+    have ih := in_val_then_val_slice hv
+    simp [Value.sliceEUIDs]
+    rw [mem_flatten_union_iff_mem_any]
+    exists v.sliceEUIDs
+    simp only [ih, List.mem_map, Subtype.exists, Prod.exists, and_true]
+    exists a, v
+    simp [Map.find?_mem_toList, ha]
+  case set | ext =>
+    unfold EuidInValue at hv
+    split at hv <;> split at hv <;>
+    ( rename_i hv' ; simp at hv hv' )
+
+theorem slice_at_succ_n_reachable {e : Expr} {n : Nat} {c c' : Capabilities} {tx : TypedExpr} {env : Environment} {entities : Entities}
+  (hc : CapabilitiesInvariant c request entities)
+  (hr : RequestAndEntitiesMatchEnvironment env request entities)
+  (ht : typeOf e c env = .ok (tx, c'))
+  (hl : checkLevel tx n = LevelCheckResult.mk true true)
+  (he : evaluate e request entities = .ok v)
+  (ha : ∃ attrs, EuidInValue v attrs euid )
+  (hf : entities.contains euid) :
+  ReachableIn entities request.sliceEUIDs euid (1 + n)
+:= by
+  cases e
+  case lit =>
+    simp [evaluate] at he
+    subst he
+    unfold EuidInValue at ha
+    replace ⟨ attrs, ha ⟩ := ha
+    split at ha <;> try simp at ha
+    split at ha <;> try simp at ha
+    subst ha
+    rename_i hp
+    injections hp
+    subst hp
+    simp [typeOf, typeOfLit] at ht
+    split at ht
+    case isTrue =>
+      simp [ok] at ht
+      replace ⟨ ht, hc' ⟩ := ht
+      subst ht hc'
+      simp [checkLevel] at hl
+    case isFalse =>
+      simp [err] at ht
+  case var v =>
+    cases v <;> simp [evaluate] at he
+    case context =>
+      subst he
+      unfold ReachableIn
+      simp
+      left
+      rw [Request.sliceEUIDs, Set.mem_union_iff_mem_or, ←Set.make_mem]
+      right
+      simp [Value.sliceEUIDs]
+      unfold EuidInValue at ha
+      replace ⟨ attrs, ha ⟩ := ha
+      simp at ha
+      split at ha <;> try contradiction
+      split at ha <;> try contradiction
+      rename_i hctx
+      have ha' := in_val_then_val_slice ha
+      rename_i a _ _ v
+      rw [mem_flatten_union_iff_mem_any]
+      exists v.sliceEUIDs
+      simp [ha']
+      exists a, v
+      simp
+      exact Map.find?_mem_toList hctx
+    all_goals {
+      subst he
+      unfold ReachableIn
+      rw [Request.sliceEUIDs, Set.mem_union_iff_mem_or, ←Set.make_mem]
+      unfold EuidInValue at ha
+      replace ⟨ attrs, ha ⟩ := ha
+      split at ha <;> try contradiction
+      simp [ha]
+    }
+  case getAttr e a =>
+    simp [evaluate] at he
+    cases h₁ : evaluate e request entities <;> simp [h₁] at he
+    have ⟨ hc', tx', c₁', ht', htx, h₂ ⟩ := type_of_getAttr_inversion ht
+    subst hc'
+    rw [htx] at hl
+    simp only [checkLevel, gt_iff_lt] at hl
+    have ⟨ hgc, v, he', hi ⟩ := type_of_is_sound hc hr ht'
+    split at hl
+    · rename_i hety
+      simp at hl
+      have ⟨⟨⟨hl₀, hl₁⟩, hl₂⟩, hl₃⟩ := hl ; clear hl
+      have hl' : checkLevel tx' (n - 1) = LevelCheckResult.mk true true := by
+        have h : ∀ r, r = LevelCheckResult.mk r.checked r.root := by simp
+        rw [h (checkLevel tx' (n - 1))]
+        simp [hl₂, hl₃]
+      rw [hety] at hi
+      have ⟨ euid', hety, hv⟩  := instance_of_entity_type_is_entity hi
+      subst hety hv
+      unfold EvaluatesTo at he'
+      rw [h₁] at he'
+      cases he' <;> rename_i he' <;> simp at he'
+      subst he'
+
+      simp [getAttr, attrsOf] at he
+      cases h₅ : entities.attrs euid' <;> simp [h₅] at he
+      rename_i attrs
+      simp [Map.findOrErr] at he
+      split at he <;> simp at he
+      subst he
+      rename_i v hv
+
+      have ⟨ ed, hed, hed' ⟩ := entities_attrs_then_find? h₅
+      subst attrs
+      have hf' : entities.contains euid' := by simp [Map.contains, Option.isSome, hed]
+
+      have ih := slice_at_succ_n_reachable hc hr ht' hl' h₁ (by exists []) hf'
+      have h₆ : (1 + (n - 1)) = n := by omega
+      rw [h₆] at ih ; clear h₆
+
+      symm at hv hed
+      apply reachable_attr_step ih hed hv ha
+
+    · rename_i hty
+      cases h₂ <;> rename_i h₂
+      · replace ⟨ ety, h₂ ⟩ := h₂
+        specialize hty ety h₂
+        contradiction
+      · replace ⟨ rty, h₂ ⟩ := h₂
+        clear hty
+        rw [h₂] at hi
+        have ⟨ attrs, hv⟩ := instance_of_record_type_is_record hi ; clear hi
+        subst hv
+        unfold EvaluatesTo at he'
+        rw [h₁] at he'
+        cases he' <;> rename_i he' <;> simp at he'
+        subst he'
+        simp [getAttr, attrsOf, Map.findOrErr] at he
+        split at he <;> simp at he
+        rename_i v hv
+        subst he
+        replace ⟨ path, ha ⟩ := ha
+        have ha' : ∃ path', EuidInValue (Value.record attrs) path' euid := by
+          exists a :: path
+          simp [EuidInValue, hv, ha]
+        exact slice_at_succ_n_reachable hc hr ht' hl h₁ ha' hf
+  all_goals { sorry }
+
+-- Because e typechecked and was annotated as ty₁ which then level checked
+-- at level (n - 1), we know that `euid` is the result of at most `n - 1`
+-- dereferences. `slice` was taken from `entities` at level `n`, so we can
+-- do at least one more dereference without error.
+theorem slice_at_succ_n_has_entity  {n : Nat} {c c' : Capabilities} {tx : TypedExpr} {env : Environment} {slice entities : Entities} {ed : EntityData}
+  (hs : slice = Entities.sliceAtLevel entities request (1 + n))
+  (hc : CapabilitiesInvariant c request entities)
+  (hr : RequestAndEntitiesMatchEnvironment env request entities)
+  (ht : typeOf e c env = .ok (tx, c'))
+  (hl : checkLevel tx n = LevelCheckResult.mk true true)
+  (he : evaluate e request entities = .ok (Value.prim (Prim.entityUID euid)))
+  (hf : entities.find? euid = some ed) :
+  slice.find? euid = some ed
+:= by
+  simp [Entities.sliceAtLevel] at hs
+  cases h₁ : Entities.sliceAtLevel.sliceAtLevel entities request.sliceEUIDs (1 + n)  <;> simp [h₁] at hs
+  rename_i eids
+  cases h₂ : (List.mapM (fun e => (Map.find? entities e).bind fun __do_lift => some (e, __do_lift)) eids.elts)  <;> simp [h₂] at hs
+  subst hs
+  cases e
+  case lit =>
+    simp [evaluate] at he
+    subst he
+    simp [typeOf, typeOfLit] at ht
+    split at ht
+    case isTrue =>
+      simp [ok] at ht
+      replace ⟨ ht, hc' ⟩ := ht
+      subst ht hc'
+      simp [checkLevel] at hl
+    case isFalse =>
+      simp [err] at ht
+  case var v =>
+    cases v <;> simp [evaluate] at he
+    all_goals {
+      have hw : ReachableIn entities request.sliceEUIDs euid (1 + n) := by
+        unfold ReachableIn ; simp
+        left
+        simp [←he, Request.sliceEUIDs]
+        rw [Set.mem_union_iff_mem_or]
+        left
+        rw [←Set.make_mem]
+        simp
+      subst he
+      symm at h₁
+      have hi := slice_contains_reachable hw h₁ (by simp [hf, Map.contains_iff_some_find?])
+      rw [←hf]
+      symm at h₂
+      exact map_find_mapm_value h₂ hi
+    }
+  case getAttr e a =>
+    have hv : ∃ path, EuidInValue (Value.prim (Prim.entityUID euid)) path euid := by exists []
+    have hf' : Map.contains entities euid := by simp [Map.contains, hf]
+    have hw : ReachableIn entities request.sliceEUIDs euid (1 + n) :=
+      slice_at_succ_n_reachable hc hr ht hl he hv hf'
+    symm at h₁
+    have hi := slice_contains_reachable hw h₁ (by simp [hf, Map.contains_iff_some_find?])
+    rw [←hf]
+    symm at h₂
+    exact map_find_mapm_value h₂ hi
+  all_goals { sorry }
+
+theorem level_based_slicing_is_sound {e : Expr} {n : Nat} {c : Capabilities} {env : Environment} {request : Request} {slice entities : Entities}
+  (hs : slice = entities.sliceAtLevel request n)
   (hc : CapabilitiesInvariant c request entities)
   (h₂ : RequestAndEntitiesMatchEnvironment env request entities)
-  (h₁ : typedAtLevel e c env 0) :
-  evaluate e request entities = evaluate e request Map.empty
+  (h₁ : typedAtLevel e c env n) :
+  evaluate e request entities = evaluate e request slice
 := by
-  have ⟨_, _, h₃, h₄⟩ := typed_at_level_inversion h₁
+  replace ⟨_, _, h₃, h₁⟩ := typed_at_level_inversion h₁
   cases e
   case lit => simp [evaluate]
   case var v => cases v <;> simp [evaluate]
   case ite c t e =>
-    have ihc := @level_based_slicing_is_sound₀ c
-    have iht := @level_based_slicing_is_sound₀ t
-    have ihe := @level_based_slicing_is_sound₀ e
-    apply level_based_slicing_is_sound_if₀ hc h₂ h₃ h₄ ihc iht ihe
-  case and => sorry
-  case or => sorry
-  case unaryApp => sorry
-  case binaryApp => sorry
-  case getAttr => sorry
-  case hasAttr => sorry
-  case set => sorry
-  case record => sorry
-  case call => sorry
-
--- theorem level_based_slicing_is_sound' {e : Expr} {env : Environment} {request : Request} {entities slice : Entities} {n : Nat} :
---   slice = entities.sliceAtLevel request n →
---   typedAtLevel e env n →
---   evaluate e request entities = evaluate e request slice
--- := by
---   intros h₁ h₂
---   cases n
---   ·
---     simp [Entities.sliceAtLevel, Entities.sliceAtLevel.sliceAtLevel, Map.make, List.canonicalize] at h₁
---     subst slice
---     simp [typedAtLevel] at h₂
---     split at h₂ <;> try simp at h₂
---     -- unfold checkLevel at h₂
-
-
-
-/-
-theorem level_based_slicing_is_sound {e : Expr} {env : Environment} {request : Request} {entities slice : Entities} {n : Nat} :
-  slice = entities.sliceAtLevel request n →
-  typedAtLevel e env n →
-  evaluate e request entities = evaluate e request slice
-:= by
-  intros h₁
-  cases e
-  case lit =>
-    simp [evaluate]
-  case var v =>
-    cases v <;> simp [evaluate]
-  case ite c t e =>
-    intros h₂
-    have ⟨_, _, h₃, h₄⟩ := typed_at_level_then_type_and_level h₂
-    have ⟨ty₁, bty₁, c₁, ty₂, c₂, ty₃, c₃, h₅, h₆, h₇ ⟩  := type_of_ite_inversion h₃
-    split at h₇
-    · replace ⟨h₇, h₈, h₉⟩ := h₇
-      subst c₃ ty₃
-      have h₁₀ : typedAtLevel e env n := by sorry
-      have h₁₁ := level_based_slicing_is_sound h₁ h₁₀
-      have hc := empty_capabilities_invariant request entities
-      have ⟨ hgc, v, h₁₂, h₁₃ ⟩ := type_of_is_sound hc (by sorry) h₅
-      have hc' := empty_capabilities_invariant request slice
-      have ⟨ hgc', v', h'₁₂, h'₁₃ ⟩ := type_of_is_sound hc' (by sorry) h₅
-      rw [h₆] at h₁₃
-      rw [h₆] at h'₁₃
-      have h₁₄ := instance_of_ff_is_false h₁₃
-      have h'₁₄ := instance_of_ff_is_false h'₁₃
-      subst v v'
+    have ihc := @level_based_slicing_is_sound c
+    have iht := @level_based_slicing_is_sound t
+    have ihe := @level_based_slicing_is_sound e
+    apply level_based_slicing_is_sound_if hs hc h₂ h₃ h₁ ihc iht ihe
+  case and => sorry -- inductive case, similar ast rewriting concerns as `if`
+  case or => sorry -- inductive case, similar ast rewriting concerns as `if`
+  case unaryApp => sorry -- trivial inductive cases
+  case binaryApp => sorry -- includes tags cases which should follow the attr cases and `in` case which might be tricky
+  case getAttr e a =>
+    have ⟨ h₇, ty₁, c₁', h₄, h₅, h₆ ⟩ := type_of_getAttr_inversion h₃
+    subst h₇
+    cases h₆
+    case _ h₇ =>
+      replace ⟨ ety, h₇⟩ := h₇
+      have ⟨ hgc, v, h₁₃, h₁₄ ⟩ := type_of_is_sound hc h₂ h₄
+      rw [h₇] at h₁₄
+      replace ⟨ euid, h₁₄, h₁₅⟩ := instance_of_entity_type_is_entity h₁₄
+      subst h₁₄ h₁₅
+      rw [h₅] at h₁
+      simp [checkLevel, h₇] at h₁
+      have ⟨ ⟨ hll₁, hl₁⟩, hr₁ ⟩ := h₁ ; clear h₁
+      have h₈ := check_level_succ hr₁
+      have h₉ : (1 + (n - 1)) = n := by omega
+      rw [h₉] at h₈ ; clear h₉
       simp [evaluate]
-      cases h₁₂ <;> cases h'₁₂
-      · rename_i h₁₂ h'₁₂
-        rw [h₁₂, h'₁₂]
-        simp [Result.as]
-      · rename_i h₁₂ h'₁₂
-        cases h₁₂ <;> cases h'₁₂
-      · sorry
-      · sorry
+      rw [←level_based_slicing_is_sound hs hc h₂ (typed_at_level_def h₄ h₈)]
+      clear h₈
+      simp [getAttr, attrsOf]
+      unfold EvaluatesTo at h₁₃
+      rcases h₁₃ with h₁₃ | h₁₃ | h₁₃ | h₁₃ <;> simp [h₁₃]
+      cases hee : entities.attrs euid
+      case error => simp [not_entities_attrs_then_not_slice_attrs hs hee]
+      case ok =>
+        have h₆ : (checkLevel ty₁ (n - 1) = LevelCheckResult.mk true true) := by
+          have h₇ : ∀ r, r = LevelCheckResult.mk r.checked r.root := by simp
+          rw [h₇ (checkLevel ty₁ (n - 1))]
+          simp [hr₁, hll₁]
+        have h₈ : n = 1 + (n - 1) := by omega
+        rw [h₈] at hs
 
-
-
-
-
-
-
-
-
-      unfold EvaluatesTo at h₁₂
-
-
-    simp [evaluate]
-    intros h₂
-    simp [typedAtLevel] at h₂
-    split at h₂
-
-
-    cases h₂ : evaluate c request entities <;>
-    cases h₃ : evaluate c request slice <;>
-    simp [Result.as, bind, Except.bind]
-    case error.ok =>
-      unfold typedAtLevel
-      cases h₄ : typeOf (c.ite t e) ∅ env <;> simp
-      intros
-      have ih := level_based_slicing_is_sound h₁
-
-
-
-    --case error.error =>
-    --  unfold typedAtLevel
-    --  cases h₄ : typeOf (c.ite t e) ∅ env
-    --  case error => simp
-    --  case ok =>
-    --    simp ; intros
-
-
-
-  case and => sorry
-  case or => sorry
-  case unaryApp => sorry
-  case binaryApp => sorry
-  case getAttr => sorry
-  case hasAttr => sorry
-  case set => sorry
-  case record => sorry
-  case call => sorry
-
--/
+        have ⟨ ed, hee', hee''⟩ := entities_attrs_then_find? hee
+        subst hee''
+        have h₇ := slice_at_succ_n_has_entity hs hc h₂ h₄ h₆ h₁₃ hee'
+        replace h₇ := entities_find?_then_attrs h₇
+        simp [h₇]
+    case _ h₇  => sorry -- record case for `getAttr`
+  case hasAttr => sorry -- should follow `getAttr`
+  case set => sorry -- trivial recursive case maybe a little tricky
+  case record => sorry -- likely to be tricky. Record cases are always hard, and here there might be an odd interaction with attribute access
+  case call => sorry -- should be the same as set
