cedar-lean/Cedar/Thm/Validation/Typechecker/IfThenElse.lean
@@ -28,19 +28,19 @@ open Cedar.Validation
 theorem type_of_ite_inversion {x₁ x₂ x₃ : Expr} {c c' : Capabilities} {env : Environment} {ty : TypedExpr}
   (h₁ : typeOf (Expr.ite x₁ x₂ x₃) c env = Except.ok (ty, c')) :
   ∃ ty₁ bty₁ c₁ ty₂ c₂ ty₃ c₃,
+    ty = TypedExpr.ite ty₁ ty₂ ty₃ ty.typeOf ∧
     typeOf x₁ c env = .ok (ty₁, c₁) ∧
     ty₁.typeOf = .bool bty₁ ∧
     match bty₁ with
     | .ff      =>
       typeOf x₃ c env = .ok (ty₃, c₃) ∧
-      ty = TypedExpr.ite ty₁ ty₃ ty₃ ty₃.typeOf ∧ c' = c₃
+      ty.typeOf = ty₃.typeOf ∧ c' = c₃
     | .tt      =>
       typeOf x₂ (c ∪ c₁) env = .ok (ty₂, c₂) ∧
-      ty = TypedExpr.ite ty₁ ty₂ ty₂ ty₂.typeOf ∧ c' = c₁ ∪ c₂
+      ty.typeOf = ty₂.typeOf ∧ c' = c₁ ∪ c₂
     | .anyBool =>
       typeOf x₂ (c ∪ c₁) env = .ok (ty₂, c₂) ∧
       typeOf x₃ c env = .ok (ty₃, c₃) ∧
-      ty = TypedExpr.ite ty₁ ty₂ ty₃ ty.typeOf ∧
       (ty₂.typeOf ⊔ ty₃.typeOf) = (.some ty.typeOf) ∧ c' = (c₁ ∪ c₂) ∩ c₃
 := by
   simp [typeOf] at h₁
@@ -54,9 +54,9 @@ theorem type_of_ite_inversion {x₁ x₂ x₃ : Expr} {c c' : Capabilities} {env
     cases h₃ : typeOf x₂ (c ∪ res₁.snd) env <;> simp [h₃] at h₁
     rename_i res₂ ; simp [ok] at h₁
     have ⟨ht₂, hc₂⟩ := h₁
-    exists res₂.fst, res₂.snd
     subst ht₂ hc₂
-    simp [h₃, ←hr₁]
+    simp [h₃, ←hr₁, TypedExpr.typeOf]
+    exists res₂.snd
   case ok.h_2 =>
     exists res₁.fst, BoolType.ff, res₁.snd
     simp [hr₁]
@@ -65,7 +65,7 @@ theorem type_of_ite_inversion {x₁ x₂ x₃ : Expr} {c c' : Capabilities} {env
     simp [ok] at h₁
     replace ⟨hl₁, hr₁⟩ := h₁
     subst hl₁ hr₁
-    exists res₃.fst
+    exists res₃.fst, res₃.fst
   case ok.h_3 =>
     exists res₁.fst, BoolType.anyBool, res₁.snd
     simp [hr₁]
@@ -77,7 +77,9 @@ theorem type_of_ite_inversion {x₁ x₂ x₃ : Expr} {c c' : Capabilities} {env
     subst ht hc
     exists res₂.fst, res₂.snd
     simp only [←hr₁, h₃, Except.ok.injEq, true_and]
-    exists res₃.fst, res₃.snd
+    exists res₃.fst
+    simp [TypedExpr.typeOf]
+    exists res₃.snd
 
 theorem type_of_ite_is_sound {x₁ x₂ x₃ : Expr} {c₁ c₂ : Capabilities} {env : Environment} {ty : TypedExpr} {request : Request} {entities : Entities}
   (h₁ : CapabilitiesInvariant c₁ request entities)
@@ -89,21 +91,21 @@ theorem type_of_ite_is_sound {x₁ x₂ x₃ : Expr} {c₁ c₂ : Capabilities} 
   GuardedCapabilitiesInvariant (Expr.ite x₁ x₂ x₃) c₂ request entities ∧
   ∃ v, EvaluatesTo (Expr.ite x₁ x₂ x₃) request entities v ∧ InstanceOfType v ty.typeOf
 := by
-  have ⟨ty₁, bty₁, rc₁, ty₂, rc₂, ty₃, rc₃, h₄, h₅, h₆⟩ := type_of_ite_inversion h₃
-  specialize ih₁ h₁ h₂ h₄
+  have ⟨ty₁, bty₁, rc₁, ty₂, rc₂, ty₃, rc₃, h₄, h₅, h₆, h₇⟩ := type_of_ite_inversion h₃
+  specialize ih₁ h₁ h₂ h₅
   have ⟨ih₁₁, v₁, ih₁₂, ih₁₃⟩ := ih₁
-  simp [h₅] at ih₁₃
+  simp [h₆] at ih₁₃
   have ⟨b₁, hb₁⟩ := instance_of_bool_is_bool ih₁₃
   subst hb₁
-  cases bty₁ <;> simp at h₆
+  cases bty₁ <;> simp at h₇
   case anyBool =>
-    have ⟨h₅, h₆, ht, hty, hc⟩ := h₆
+    have ⟨h₈, ht, hty, hc⟩ := h₇
     cases b₁
     case false =>
       rcases ih₁₂ with ih₁₂ | ih₁₂ | ih₁₂ | ih₁₂ <;>
       simp [EvaluatesTo, evaluate, Result.as, ih₁₂, Coe.coe, Value.asBool, GuardedCapabilitiesInvariant] <;>
       try exact type_is_inhabited ty.typeOf
-      specialize ih₃ h₁ h₂ h₆
+      specialize ih₃ h₁ h₂ ht
       have ⟨ih₃₁, v₃, ih₃₂, ih₃₃⟩ := ih₃
       rcases ih₃₂ with ih₃₂ | ih₃₂ | ih₃₂ | ih₃₂ <;> simp [ih₃₂] <;>
       try exact type_is_inhabited ty.typeOf
@@ -122,7 +124,7 @@ theorem type_of_ite_is_sound {x₁ x₂ x₃ : Expr} {c₁ c₂ : Capabilities} 
       try exact type_is_inhabited ty.typeOf
       simp [GuardedCapabilitiesInvariant, ih₁₂] at ih₁₁
       have h₇ := capability_union_invariant h₁ ih₁₁
-      specialize ih₂ h₇ h₂ h₅
+      specialize ih₂ h₇ h₂ h₈
       have ⟨ih₂₁, v₂, ih₂₂, ih₂₃⟩ := ih₂
       apply And.intro
       case left =>
@@ -138,7 +140,7 @@ theorem type_of_ite_is_sound {x₁ x₂ x₃ : Expr} {c₁ c₂ : Capabilities} 
         apply instance_of_lub hty
         simp [ih₂₃]
   case tt =>
-    have ⟨h₅, ht, hc⟩ := h₆
+    replace ⟨h₇, ht, hc⟩ := h₇
     rcases ih₁₂ with ih₁₂ | ih₁₂ | ih₁₂ | ih₁₂ <;>
     simp [EvaluatesTo, evaluate, Result.as, ih₁₂, Coe.coe, Value.asBool, GuardedCapabilitiesInvariant] <;>
     try exact type_is_inhabited ty.typeOf
@@ -146,26 +148,26 @@ theorem type_of_ite_is_sound {x₁ x₂ x₃ : Expr} {c₁ c₂ : Capabilities} 
     simp at hb₁ ; subst hb₁ ; simp only [ite_true]
     simp [GuardedCapabilitiesInvariant, ih₁₂] at ih₁₁
     have h₆ := capability_union_invariant h₁ ih₁₁
-    specialize ih₂ h₆ h₂ h₅
+    specialize ih₂ h₆ h₂ h₇
     have ⟨ih₂₁, v₂, ih₂₂, ih₂₃⟩ := ih₂
     rcases ih₂₂ with ih₂₂ | ih₂₂ | ih₂₂ | ih₂₂ <;> simp [ih₂₂] <;>
     try exact type_is_inhabited ty.typeOf
-    unfold TypedExpr.typeOf
-    subst ht hc
-    simp [ih₂₃]
+    subst hc
+    simp [ht, ih₂₃]
     intro h₇ ; subst h₇
     simp [GuardedCapabilitiesInvariant, ih₂₂] at ih₂₁
     exact capability_union_invariant ih₁₁ ih₂₁
   case ff =>
-    have ⟨h₅, ht, hc⟩ := h₆
+    replace ⟨h₇, ht, hc⟩ := h₇
     rcases ih₁₂ with ih₁₂ | ih₁₂ | ih₁₂ | ih₁₂ <;>
     simp [EvaluatesTo, evaluate, Result.as, ih₁₂, Coe.coe, Value.asBool, GuardedCapabilitiesInvariant] <;>
     try exact type_is_inhabited ty.typeOf
     have hb₁ := instance_of_ff_is_false ih₁₃
     simp at hb₁ ; simp [hb₁]
-    specialize ih₃ h₁ h₂ h₅
+    specialize ih₃ h₁ h₂ h₇
     have ⟨ih₃₁, v₃, ih₃₂, ih₃₃⟩ := ih₃
-    subst hc ht
+    subst hc
+    rw [ht]
     apply And.intro
     · simp [GuardedCapabilitiesInvariant] at ih₃₁
       exact ih₃₁
